library/data/rbtree/find.lean
@@ -47,16 +47,16 @@ begin
       apply iff.intro,
       {
         intro hm, blast_disjs,
-        { exact iff.mp (ih hs₁) hm },
+        { exact iff.mp (ih hs_hs₁) hm },
         { simp at h, cases hm, contradiction },
         {
-          have hyx : lift lt (some y) (some x) := (range hs₂ hm).1,
+          have hyx : lift lt (some y) (some x) := (range hs_hs₂ hm).1,
           simp [lift] at hyx,
           have hxy : lt x y, { simp [cmp_using] at h, assumption },
           exact absurd (trans_of lt hxy hyx) (irrefl_of lt x)
         }
       },
-      { intro hc, left, exact iff.mpr (ih hs₁) hc },
+      { intro hc, left, exact iff.mpr (ih hs_hs₁) hc },
     },
     { simp at h, simp [h, strict_weak_order.equiv], existsi y, split, refl, assumption },
     {
@@ -65,22 +65,22 @@ begin
       {
         intro hm, blast_disjs,
         {
-          have hxy : lift lt (some x) (some y) := (range hs₁ hm).2,
+          have hxy : lift lt (some x) (some y) := (range hs_hs₁ hm).2,
           simp [lift] at hxy,
           have hyx : lt y x, { simp [cmp_using] at h, exact h.2 },
           exact absurd (trans_of lt hxy hyx) (irrefl_of lt x)
         },
         { simp at h, cases hm, contradiction },
-        { exact iff.mp (ih hs₂) hm }
+        { exact iff.mp (ih hs_hs₂) hm }
       },
-      { intro hc, right, right, exact iff.mpr (ih hs₂) hc },
+      { intro hc, right, right, exact iff.mpr (ih hs_hs₂) hc },
     } }
 end
 
 lemma mem_of_mem_exact {lt} [is_irrefl α lt] {x t} : mem_exact x t → mem lt x t :=
 begin
   induction t; simp [mem_exact, mem]; intro h,
-  all_goals { blast_disjs, simp [ih_1 h], simp [h, irrefl_of lt val], simp [ih_2 h] }
+  all_goals { blast_disjs, simp [t_ih_1 h], simp [h, irrefl_of lt t_val], simp [t_ih_2 h] }
 end
 
 lemma find_correct_exact {t : rbnode α} {lt x} [decidable_rel lt] [is_strict_weak_order α lt] : ∀ {lo hi} (hs : is_searchable lt t lo hi), mem_exact x t ↔ find lt t x = some x :=
@@ -93,26 +93,26 @@ begin
       apply iff.intro,
       {
         intro hm, blast_disjs,
-        { exact iff.mp (ih hs₁) hm },
+        { exact iff.mp (ih hs_hs₁) hm },
         { simp at h, subst x, exact absurd h (irrefl y) },
-        { have hyx : lift lt (some y) (some x) := (range hs₂ (mem_of_mem_exact hm)).1,
+        { have hyx : lift lt (some y) (some x) := (range hs_hs₂ (mem_of_mem_exact hm)).1,
           simp [lift] at hyx,
           have hxy : lt x y, { simp [cmp_using] at h, assumption },
           exact absurd (trans_of lt hxy hyx) (irrefl_of lt x)
         }
       },
-      { intro hc, left, exact iff.mpr (ih hs₁) hc },
+      { intro hc, left, exact iff.mpr (ih hs_hs₁) hc },
     },
     { simp at h,
       cases hs,
       apply iff.intro,
       {
         intro hm, blast_disjs,
-        { have hxy : lift lt (some x) (some y) := (range hs₁ (mem_of_mem_exact hm)).2,
+        { have hxy : lift lt (some x) (some y) := (range hs_hs₁ (mem_of_mem_exact hm)).2,
           simp [lift] at hxy,
           exact absurd hxy h.1 },
         { subst hm },
-        { have hyx : lift lt (some y) (some x) := (range hs₂ (mem_of_mem_exact hm)).1,
+        { have hyx : lift lt (some y) (some x) := (range hs_hs₂ (mem_of_mem_exact hm)).1,
           simp [lift] at hyx,
           exact absurd hyx h.2 } },
       { intro hm, injection hm, simp [*] } },
@@ -122,15 +122,15 @@ begin
       {
         intro hm, blast_disjs,
         {
-          have hxy : lift lt (some x) (some y) := (range hs₁ (mem_of_mem_exact hm)).2,
+          have hxy : lift lt (some x) (some y) := (range hs_hs₁ (mem_of_mem_exact hm)).2,
           simp [lift] at hxy,
           have hyx : lt y x, { simp [cmp_using] at h, exact h.2 },
           exact absurd (trans_of lt hxy hyx) (irrefl_of lt x)
         },
         { simp at h, subst x, exact absurd h (irrefl y) },
-        { exact iff.mp (ih hs₂) hm }
+        { exact iff.mp (ih hs_hs₂) hm }
       },
-      { intro hc, right, right, exact iff.mpr (ih hs₂) hc } } }
+      { intro hc, right, right, exact iff.mpr (ih hs_hs₂) hc } } }
 end
 
 lemma eqv_of_find_some {t : rbnode α} {lt x y} [decidable_rel lt] [is_strict_weak_order α lt] : ∀ {lo hi} (hs : is_searchable lt t lo hi) (he : find lt t x = some y), x ≈[lt] y :=
@@ -138,9 +138,9 @@ begin
   apply find.induction lt t x; intros; simp only [mem, find, *] at *,
   { contradiction },
   iterate 2 {
-    { cases hs, exact ih hs₁ rfl },
+    { cases hs, exact ih hs_hs₁ rfl },
     { injection he, subst y, simp at h, exact h },
-    { cases hs, exact ih hs₂ rfl } }
+    { cases hs, exact ih hs_hs₂ rfl } }
 end
 
 lemma find_eq_find_of_eqv {lt a b} [decidable_rel lt] [is_strict_weak_order α lt] {t : rbnode α} : ∀ {lo hi} (hs : is_searchable lt t lo hi) (heqv : a ≈[lt] b), find lt t a = find lt t b :=
@@ -148,11 +148,11 @@ begin
   apply find.induction lt t a; intros; simp [mem, find, strict_weak_order.equiv, *] at *,
   iterate 2 {
     { have : lt b y := lt_of_incomp_of_lt heqv.swap h,
-      simp [cmp_using, find, *], cases hs, apply ih hs₁ },
+      simp [cmp_using, find, *], cases hs, apply ih hs_hs₁ },
     { have := incomp_trans_of lt heqv.swap h, simp [cmp_using, find, *] },
     { have := lt_of_lt_of_incomp h heqv,
       have := not_lt_of_lt this,
-      simp [cmp_using, find, *], cases hs, apply ih hs₂ } }
+      simp [cmp_using, find, *], cases hs, apply ih hs_hs₂ } }
 end
 
 end rbnode
