library/data/rbtree/min_max.lean
@@ -14,9 +14,9 @@ begin
    induction t,
    { intros, contradiction },
    all_goals {
-     cases lchild; simp [rbnode.min]; intro h,
-     { injection h, subst val, simp [mem, irrefl_of lt a] },
-     all_goals { rw [mem], simp [ih_1 h] } }
+     cases t_lchild; simp [rbnode.min]; intro h,
+     { injection h, subst t_val, simp [mem, irrefl_of lt a] },
+     all_goals { rw [mem], simp [t_ih_1 h] } }
 end
 
 lemma mem_of_max_eq (lt : α → α → Prop) [is_irrefl α lt] {a : α} {t : rbnode α} : t.max = some a → mem lt a t :=
@@ -24,9 +24,9 @@ begin
    induction t,
    { intros, contradiction },
    all_goals {
-     cases rchild; simp [rbnode.max]; intro h,
-     { injection h, subst val, simp [mem, irrefl_of lt a] },
-     all_goals { rw [mem], simp [ih_2 h] } }
+     cases t_rchild; simp [rbnode.max]; intro h,
+     { injection h, subst t_val, simp [mem, irrefl_of lt a] },
+     all_goals { rw [mem], simp [t_ih_2 h] } }
 end
 
 variables [decidable_rel lt] [is_strict_weak_order α lt]
@@ -36,9 +36,9 @@ begin
   induction t,
   { intros, refl },
   all_goals {
-    cases lchild; simp [rbnode.min]; intro h,
+    cases t_lchild; simp [rbnode.min]; intro h,
     { contradiction },
-    all_goals { have := ih_1 h, contradiction } }
+    all_goals { have := t_ih_1 h, contradiction } }
 end
 
 lemma eq_leaf_of_max_eq_none {t : rbnode α} : t.max = none → t = leaf :=
@@ -46,9 +46,9 @@ begin
   induction t,
   { intros, refl },
   all_goals {
-    cases rchild; simp [rbnode.max]; intro h,
+    cases t_rchild; simp [rbnode.max]; intro h,
     { contradiction },
-    all_goals { have := ih_2 h, contradiction } }
+    all_goals { have := t_ih_2 h, contradiction } }
 end
 
 lemma min_is_minimal {a : α} {t : rbnode α} : ∀ {lo hi}, is_searchable lt t lo hi → t.min = some a → ∀ {b}, mem lt b t → a ≈[lt] b ∨ lt a b :=
@@ -56,8 +56,8 @@ begin
   induction t,
   { simp [strict_weak_order.equiv], intros _ _ hs hmin b, contradiction },
   all_goals {
-    cases lchild; intros lo hi hs hmin b hmem,
-    { simp [rbnode.min] at hmin, injection hmin, subst val,
+    cases t_lchild; intros lo hi hs hmin b hmem,
+    { simp [rbnode.min] at hmin, injection hmin, subst t_val,
       simp [mem] at hmem, cases hmem with heqv hmem,
       { left, exact heqv.swap },
       { have := lt_of_mem_right hs (by constructor) hmem,
@@ -66,7 +66,7 @@ begin
       have hs' := hs,
       cases hs, simp [rbnode.min] at hmin,
       rw [mem] at hmem, blast_disjs,
-      { exact ih_1 hs₁ hmin hmem },
+      { exact t_ih_1 hs_hs₁ hmin hmem },
       { have hmm       := mem_of_min_eq lt hmin,
         have a_lt_val  := lt_of_mem_left hs' (by constructor) hmm,
         have a_lt_b    := lt_of_lt_of_incomp a_lt_val hmem.swap,
@@ -81,8 +81,8 @@ begin
   induction t,
   { simp [strict_weak_order.equiv], intros _ _ hs hmax b, contradiction },
   all_goals {
-    cases rchild; intros lo hi hs hmax b hmem,
-    { simp [rbnode.max] at hmax, injection hmax, subst val,
+    cases t_rchild; intros lo hi hs hmax b hmem,
+    { simp [rbnode.max] at hmax, injection hmax, subst t_val,
       simp [mem] at hmem, cases hmem with hmem heqv,
       { have := lt_of_mem_left hs (by constructor) hmem,
         right, assumption },
@@ -98,7 +98,7 @@ begin
         have val_lt_a  := lt_of_mem_right hs' (by constructor) hmm,
         have a_lt_b    := lt_of_incomp_of_lt hmem val_lt_a,
         right, assumption },
-      { exact ih_2 hs₂ hmax hmem } } }
+      { exact t_ih_2 hs_hs₂ hmax hmem } } }
 end
 
 end rbnode
