tests/lean/induction_naming.lean
@@ -1,0 +1,22 @@
+example (a b : nat) : a + b = b + a :=
+begin
+  cases a,
+  trace_state, /- `a` was used to name constructor field -/
+  repeat { admit }
+end
+
+example (a b : nat) : a + b = b + a :=
+begin
+  induction a,
+  trace_state, /- `a_n` and `a_ih` were used to name constructor fields -/
+  repeat { admit }
+end
+
+set_option tactic.induction.concat_names false
+
+example (a b : nat) : a + b = b + a :=
+begin
+  induction a,
+  trace_state, /- `n` and `ih` were used to name constructor fields -/
+  repeat { admit }
+end
